Changes to Rutt, IP

theories/Eq/Rutt.v
@@ -17,24 +17,18 @@
 
 From Stdlib Require Import
      Morphisms
-.
+     Program.
 
-From ExtLib Require Import
-     Structures.Monad.
+From Coinduction Require Import all.
 
 From ITree Require Import
      Basics.Utils
      Axioms
-     ITree
-     Eq
-     Basics
-.
+     Core.ITreeDefinition
+     Eq.Eqit
+     Eq.Shallow.
 
-From Paco Require Import paco.
-
-Import Monads.
-Import MonadNotation.
-Local Open Scope monad_scope.
+Local Open Scope itree_scope.
 
 Section RuttF.
 
@@ -45,58 +39,62 @@ Section RuttF.
   Contributions to that effect are welcome. *)
   Context (REv : forall (A B : Type), E1 A -> E2 B -> Prop ).
   Context (RAns : forall (A B : Type), E1 A -> A -> E2 B -> B -> Prop ).
-  Context (RR : R1 -> R2 -> Prop).
   Arguments REv {A} {B}.
   Arguments RAns {A} {B}.
 
-  Inductive ruttF (sim : itree E1 R1 -> itree E2 R2 -> Prop) : itree' E1 R1 -> itree' E2 R2 -> Prop :=
+  Inductive ruttF (RR: R1 -> R2 -> Prop) (sim : itree E1 R1 -> itree E2 R2 -> Prop) : itree' E1 R1 -> itree' E2 R2 -> Prop :=
   | EqRet : forall (r1 : R1) (r2 : R2),
       RR r1 r2 ->
-      ruttF sim (RetF r1) (RetF r2)
+      ruttF RR sim (RetF r1) (RetF r2)
   | EqTau : forall (m1 : itree E1 R1) (m2 : itree E2 R2),
       sim m1 m2 ->
-      ruttF sim (TauF m1) (TauF m2)
+      ruttF RR sim (TauF m1) (TauF m2)
   | EqVis : forall (A B : Type) (e1 : E1 A) (e2 : E2 B ) (k1 : A -> itree E1 R1) (k2 : B -> itree E2 R2),
       REv e1 e2 ->
       (forall (a : A) (b : B), RAns e1 a e2 b -> sim (k1 a) (k2 b)) ->
-      ruttF sim (VisF e1 k1) (VisF e2 k2)
+      ruttF RR sim (VisF e1 k1) (VisF e2 k2)
   | EqTauL : forall (t1 : itree E1 R1) (ot2 : itree' E2 R2),
-      ruttF sim (observe t1) ot2 ->
-      ruttF sim (TauF t1) ot2
+      ruttF RR sim (observe t1) ot2 ->
+      ruttF RR sim (TauF t1) ot2
   | EqTauR : forall (ot1 : itree' E1 R1) (t2 : itree E2 R2),
-      ruttF sim ot1 (observe t2) ->
-      ruttF sim ot1 (TauF t2).
+      ruttF RR sim ot1 (observe t2) ->
+      ruttF RR sim ot1 (TauF t2).
   Hint Constructors ruttF : itree.
 
-  Definition rutt_ (sim : itree E1 R1 -> itree E2 R2 -> Prop)
-             (t1 : itree E1 R1) (t2 : itree E2 R2) :=
-    ruttF sim (observe t1) (observe t2).
-  Hint Unfold rutt_ : itree.
+  Definition rutt_ (sim : (R1 -> R2 -> Prop) -> itree E1 R1 -> itree E2 R2 -> Prop) :
+    (R1 -> R2 -> Prop) -> itree E1 R1 -> itree E2 R2 -> Prop :=
+    fun RR t1 t2 =>
+      ruttF RR (sim RR) (observe t1) (observe t2).
 
-  Lemma rutt_monot : monotone2 rutt_.
+  Lemma rutt_mono : Proper (leq ==> leq) rutt_.
   Proof.
-    red. intros. red; induction IN; eauto with itree.
+    repeat intro. unfold rutt_ in *. induction H0; eauto with itree.
+    constructor; now apply H. 
+    constructor; intros; eauto; now apply H, H1. 
   Qed.
 
-  Definition rutt : itree E1 R1 -> itree E2 R2 -> Prop := paco2 rutt_ bot2.
+  Definition rutt_mon : mon ((R1 -> R2 -> Prop) -> itree E1 R1 -> itree E2 R2 -> Prop) :=
+    {| body := rutt_ ; Hbody := rutt_mono |}. 
+
+  Definition rutt : (R1 -> R2 -> Prop) -> itree E1 R1 -> itree E2 R2 -> Prop := gfp rutt_mon.
   Hint Unfold rutt : itree.
 
-  Lemma ruttF_inv_VisF_r {sim} t1 U2 (e2: E2 U2) (k2: U2 -> _):
-    ruttF sim t1 (VisF e2 k2) ->
+  Lemma ruttF_inv_VisF_r {sim} RR t1 U2 (e2: E2 U2) (k2: U2 -> _):
+    ruttF RR sim t1 (VisF e2 k2) ->
     (exists U1 (e1: E1 U1) k1, t1 = VisF e1 k1 /\
       forall v1 v2, RAns e1 v1 e2 v2 -> sim (k1 v1) (k2 v2))
     \/
     (exists t1', t1 = TauF t1' /\
-      ruttF sim (observe t1') (VisF e2 k2)).
+      ruttF RR sim (observe t1') (VisF e2 k2)).
   Proof.
     refine (fun H =>
-      match H in ruttF _ _ t2 return
+      match H in ruttF _ _ _ t2 return
         match t2 return Prop with
         | VisF e2 k2 => _
         | _ => True
         end
       with
-      | EqVis _ _ _ _ _ _ _ _ _ => _
+      | EqVis _ _ _ _ _ _ _ _ _ _ => _
       | _ => _
       end); try exact I.
     - left; eauto.
@@ -104,46 +102,56 @@ Section RuttF.
   Qed.
 
   Lemma ruttF_inv_VisF {sim}
-      U1 U2 (e1 : E1 U1) (e2 : E2 U2) (k1 : U1 -> _) (k2 : U2 -> _)
-    : ruttF sim (VisF e1 k1) (VisF e2 k2) ->
+      RR U1 U2 (e1 : E1 U1) (e2 : E2 U2) (k1 : U1 -> _) (k2 : U2 -> _)
+    : ruttF RR sim (VisF e1 k1) (VisF e2 k2) ->
       forall v1 v2, RAns e1 v1 e2 v2 -> sim (k1 v1) (k2 v2).
   Proof.
     intros H. dependent destruction H. assumption.
   Qed.
 
-
-  Ltac unfold_rutt :=
-    (try match goal with [|- rutt_ _ _ _ _ _ _ _ ] => red end);
-    (repeat match goal with [H: rutt_ _ _ _ _ _ _ _ |- _ ] => red in H end).
-
-  Lemma fold_ruttF:
-    forall (t1: itree E1 R1) (t2: itree E2 R2) ot1 ot2,
-    ruttF (upaco2 rutt_ bot2) ot1 ot2 ->
-    ot1 = observe t1 ->
-    ot2 = observe t2 ->
-    rutt t1 t2.
-  Proof.
-    intros * eq -> ->; pfold; auto.
-  Qed.
 End RuttF.
 
-Tactic Notation "fold_ruttF" hyp(H) :=
-  try punfold H;
-  try red in H;
-  match type of H with
-  | ruttF ?_REV ?_RANS ?_RR (upaco2 (rutt_ ?_REV ?_RANS ?_RR) bot2) ?_OT1 ?_OT2 =>
-      match _OT1 with
-      | observe _ => idtac
-      | ?_OT1 => rewrite (itree_eta' _OT1) in H
-      end;
-      match _OT2 with
-      | observe _ => idtac
-      | ?_OT2 => rewrite (itree_eta' _OT2) in H
-      end;
-      eapply fold_ruttF in H; [| eauto | eauto]
-  end.
+(** ** Rutt-specific tactics *)
 
-#[global] Hint Resolve rutt_monot : paco.
+(** [rstep] unfolds [rutt] one step, exposing the [ruttF] functor. *)
+Tactic Notation "rstep" :=
+  unfold rutt; step; cbn [rutt_mon body rutt_].
+Tactic Notation "rstep" "in" ident(h) :=
+  unfold rutt in h; step in h; cbn [rutt_mon body rutt_] in h.
+
+Ltac fold_rutt :=
+  match goal with
+  | |- context[@ruttF ?E1 ?E2 ?R1 ?R2 ?REv ?RAns ?RR] =>
+      change (@ruttF E1 E2 R1 R2 REv RAns RR) with (body (@rutt_mon E1 E2 R1 R2 REv RAns RR))
+  end.
+Ltac fold_rutt_in h :=
+  match type of h with
+  | context[@ruttF ?E1 ?E2 ?R1 ?R2 ?REv ?RAns ?RR] =>
+      change (@ruttF E1 E2 R1 R2 REv RAns RR) with (body (@rutt_mon E1 E2 R1 R2 REv RAns RR)) in h
+  end.
+Tactic Notation "runstep" := fold_rutt; unstep.
+Tactic Notation "runstep" "in" ident(h) := fold_rutt_in h; unstep in h.
+
+Local Ltac revert_one :=
+  match goal with [ H : _ |- _ ] => revert H end.
+Ltac runfold_coind :=
+  first
+    [intros ?; runfold_coind; revert_one |
+     unfold rutt].
+Tactic Notation "rcoinduction" simple_intropattern(R) simple_intropattern(H) :=
+  runfold_coind; coinduction R H; cbn [rutt_mon body rutt_].
+
+#[local] Ltac rcbn := cbn[rutt_mon body rutt_].
+#[local] Ltac rcbn_in H := cbn[rutt_mon body rutt_] in H.
+
+#[local] Tactic Notation "rcbn" "in" ident(h) := rcbn_in h. 
+#[local] Tactic Notation "rcbn" "in" "*" := cbn[rutt_mon body rutt] in *. 
+
+
+#[global] Hint Constructors ruttF : itree.
+#[global] Hint Unfold rutt_ : itree.
+#[global] Hint Unfold rutt_mon : itree.
+#[global] Hint Unfold rutt : itree.
 
 Section ConstructionInversion.
 Variables (E1 E2: Type -> Type).
@@ -155,19 +163,19 @@ Variable (RR: R1 -> R2 -> Prop).
 Lemma rutt_Ret r1 r2:
   RR r1 r2 ->
   @rutt E1 E2 R1 R2 REv RAns RR (Ret r1: itree E1 R1) (Ret r2: itree E2 R2).
-Proof. intros. pstep; constructor; auto. Qed.
+Proof. intros. rstep. constructor; auto. Qed.
 
 Lemma rutt_inv_Ret r1 r2:
   rutt REv RAns RR (Ret r1) (Ret r2) -> RR r1 r2.
 Proof.
-  intros. punfold H. inv H. eauto.
+  intros. rstep in H. inv H. eauto.
 Qed.
 
 Lemma rutt_inv_Ret_l r1 t2:
   rutt REv RAns RR (Ret r1) t2 -> exists r2, t2 ≳ Ret r2 /\ RR r1 r2.
 Proof.
-  intros Hrutt; punfold Hrutt; red in Hrutt; cbn in Hrutt.
-  setoid_rewrite (itree_eta t2). remember (RetF r1) as ot1; revert Heqot1.
+  intros Hrutt. rstep in Hrutt. rcbn in Hrutt.
+  setoid_rewrite (itree_eta t2). remember (RetF r1) as ot1; revert Heqot1.  
   induction Hrutt; intros; try discriminate.
   - inversion Heqot1; subst. exists r2. split; [reflexivity|auto].
   - destruct (IHHrutt Heqot1) as [r2 [H1 H2]]. exists r2; split; auto.
@@ -177,7 +185,7 @@ Qed.
 Lemma rutt_inv_Ret_r t1 r2:
   rutt REv RAns RR t1 (Ret r2) -> exists r1, t1 ≳ Ret r1 /\ RR r1 r2.
 Proof.
-  intros Hrutt; punfold Hrutt; red in Hrutt; cbn in Hrutt.
+  intros Hrutt. rstep in Hrutt. cbn in Hrutt.
   setoid_rewrite (itree_eta t1). remember (RetF r2) as ot2; revert Heqot2.
   induction Hrutt; intros; try discriminate.
   - inversion Heqot2; subst. exists r1. split; [reflexivity|auto].
@@ -185,37 +193,54 @@ Proof.
     rewrite <- itree_eta in H1. now rewrite tau_euttge.
 Qed.
 
+(** Helper: inversion of [ruttF] at [TauF] on the left. *)
+Lemma ruttF_inv_tau_l t1 ot2 :
+  ruttF REv RAns RR (rutt REv RAns RR) (TauF t1) ot2 ->
+  ruttF REv RAns RR (rutt REv RAns RR) (observe t1) ot2.
+Proof.
+  intros H. remember (TauF t1) as tt1.
+  induction H; try discriminate.
+  - inv Heqtt1. constructor. rstep in H. exact H.
+  - inv Heqtt1. exact H.
+  - constructor. auto.
+Qed.
+
+(** Helper: inversion of [ruttF] at [TauF] on the right. *)
+Lemma ruttF_inv_tau_r ot1 t2 :
+  ruttF REv RAns RR (rutt REv RAns RR) ot1 (TauF t2) ->
+  ruttF REv RAns RR (rutt REv RAns RR) ot1 (observe t2).
+Proof.
+  intros H. remember (TauF t2) as tt2.
+  induction H; try discriminate.
+  - inv Heqtt2. constructor. rstep in H. exact H.
+  - constructor. auto.
+  - inv Heqtt2. exact H.
+Qed.
+
 Lemma rutt_inv_Tau_l t1 t2 :
   rutt REv RAns RR (Tau t1) t2 -> rutt REv RAns RR t1 t2.
 Proof.
-  intros. punfold H. red in H. simpl in *.
-  remember (TauF t1) as tt1. genobs t2 ot2.
-  hinduction H before t1; intros; try discriminate.
-  - inv Heqtt1. pclearbot. pstep. red. simpobs. econstructor; eauto. pstep_reverse.
-  - inv Heqtt1. punfold_reverse H.
-  - red in IHruttF. pstep. red; simpobs. econstructor; eauto. pstep_reverse.
+  intros. rstep in H. rstep.
+  apply ruttF_inv_tau_l. exact H.
 Qed.
 
 Lemma rutt_add_Tau_l t1 t2 :
   rutt REv RAns RR t1 t2 -> rutt REv RAns RR (Tau t1) t2.
 Proof.
-  intros. pfold. red. cbn. constructor. pstep_reverse.
+  intros. rstep. constructor. rstep in H. exact H.
 Qed.
 
 Lemma rutt_inv_Tau_r t1 t2 :
   rutt REv RAns RR t1 (Tau t2) -> rutt REv RAns RR t1 t2.
 Proof.
-  intros. punfold H. red in H. simpl in *.
-  pstep. red. remember (TauF t2) as tt2 eqn:Ett2 in H.
-  revert t2 Ett2; induction H; try discriminate; intros; inversion Ett2; subst; auto.
-  - pclearbot. constructor. pstep_reverse.
-  - constructor. eapply IHruttF; eauto.
+  intros. rstep in H. rstep.
+  apply ruttF_inv_tau_r. exact H.
 Qed.
 
 Lemma rutt_add_Tau_r t1 t2 :
   rutt REv RAns RR t1 t2 -> rutt REv RAns RR t1 (Tau t2).
 Proof.
-  intros. pfold. red. cbn. constructor. pstep_reverse.
+  intros. rstep. constructor. rstep in H. exact H.
 Qed.
 
 Lemma rutt_inv_Tau t1 t2 :
@@ -230,8 +255,7 @@ Lemma rutt_Vis {T1 T2} (e1: E1 T1) (e2: E2 T2)
   (forall t1 t2, RAns _ _ e1 t1 e2 t2 -> rutt REv RAns RR (k1 t1) (k2 t2)) ->
   rutt REv RAns RR (Vis e1 k1) (Vis e2 k2).
 Proof.
-  intros He Hk. pstep; constructor; auto.
-  intros; left. apply Hk; auto.
+  intros He Hk. rstep. constructor; auto.
 Qed.
 
 Lemma rutt_inv_Vis_l {U1} (e1: E1 U1) k1 t2:
@@ -241,13 +265,12 @@ Lemma rutt_inv_Vis_l {U1} (e1: E1 U1) k1 t2:
     REv _ _ e1 e2 /\
     (forall v1 v2, RAns _ _ e1 v1 e2 v2 -> rutt REv RAns RR (k1 v1) (k2 v2)).
 Proof.
-  intros Hrutt; punfold Hrutt; red in Hrutt; cbn in Hrutt.
+  intros Hrutt. rstep in Hrutt. cbn in Hrutt.
   setoid_rewrite (itree_eta t2). remember (VisF e1 k1) as ot1; revert Heqot1.
   induction Hrutt; intros; try discriminate; subst.
   - inversion Heqot1; subst A. inversion_sigma; rewrite <- eq_rect_eq in *;
     subst; rename B into U2.
     exists U2, e2, k2; split. reflexivity. split; auto.
-    intros v1 v2 HAns. specialize (H0 v1 v2 HAns). red in H0. now pclearbot.
   - destruct (IHHrutt eq_refl) as (U2 & e2 & k2 & Ht0 & HAns).
     rewrite <- itree_eta in Ht0.
     exists U2, e2, k2; split; auto. now rewrite tau_eutt.
@@ -260,13 +283,12 @@ Lemma rutt_inv_Vis_r {U2} t1 (e2: E2 U2) k2:
     REv U1 U2 e1 e2 /\
     (forall v1 v2, RAns _ _ e1 v1 e2 v2 -> rutt REv RAns RR (k1 v1) (k2 v2)).
 Proof.
-  intros Hrutt; punfold Hrutt; red in Hrutt; cbn in Hrutt.
+  intros Hrutt. rstep in Hrutt. cbn in Hrutt.
   setoid_rewrite (itree_eta t1). remember (VisF e2 k2) as ot2; revert Heqot2.
   induction Hrutt; intros; try discriminate; subst.
   - inversion Heqot2; subst B. inversion_sigma; rewrite <- eq_rect_eq in *;
     subst; rename A into U1.
     exists U1, e1, k1; split. reflexivity. split; auto.
-    intros v1 v2 HAns. specialize (H0 v1 v2 HAns). red in H0. now pclearbot.
   - destruct (IHHrutt eq_refl) as (U1 & e1 & k1 & Ht0 & HAns).
     rewrite <- itree_eta in Ht0.
     exists U1, e1, k1; split; auto. now rewrite tau_eutt.
@@ -277,124 +299,8 @@ Lemma rutt_inv_Vis U1 U2 (e1: E1 U1) (e2: E2 U2)
   rutt REv RAns RR (Vis e1 k1) (Vis e2 k2) ->
   forall u1 u2, RAns U1 U2 e1 u1 e2 u2 -> rutt REv RAns RR (k1 u1) (k2 u2).
 Proof.
-  intros H u1 u2 Hans. punfold H.
-  apply ruttF_inv_VisF with (v1 := u1) (v2 := u2) in H. pclearbot; auto.
-  assumption.
+  intros H u1 u2 Hans. rstep in H.
+  exact (ruttF_inv_VisF _ _ _ _ _ _ _ _ _ H u1 u2 Hans).
 Qed.
+
 End ConstructionInversion.
-
-Section euttge_trans_clo.
-
-  Context {E1 E2 : Type -> Type} {R1 R2 : Type} (RR : R1 -> R2 -> Prop).
-
-  (* Closing a relation over itrees under [euttge].
-     Essentially the same closure as [eqit_trans_clo], but heterogeneous
-     in the interface argument [E].
-     We only define the closure under [euttge] as opposed to [eqit_trans_clo]
-     capturing closure under [eq_itree] and [eutt] at the same time, since it's
-     the only one we need.
-   *)
-
-  (* A transitivity functor *)
-  Variant euttge_trans_clo (r : itree E1 R1 -> itree E2 R2 -> Prop) :
-    itree E1 R1 -> itree E2 R2 -> Prop :=
-    eqit_trans_clo_intro t1 t2 t1' t2' RR1 RR2
-                         (EQVl: euttge RR1 t1 t1')
-                         (EQVr: euttge RR2 t2 t2')
-                         (REL: r t1' t2')
-                         (LERR1: forall x x' y, RR1 x x' -> RR x' y -> RR x y)
-                         (LERR2: forall x y y', RR2 y y' -> RR x y' -> RR x y) :
-      euttge_trans_clo r t1 t2.
-  Hint Constructors euttge_trans_clo : itree.
-
-  Lemma euttge_trans_clo_mon r1 r2 t1 t2
-        (IN : euttge_trans_clo r1 t1 t2)
-        (LE : r1 <2= r2) :
-    euttge_trans_clo r2 t1 t2.
-  Proof.
-    destruct IN; econstructor; eauto.
-  Qed.
-
-  Hint Resolve euttge_trans_clo_mon : paco.
-
-End euttge_trans_clo.
-
-(*replicate this proof for the models functor*)
-(* Validity of the up-to [euttge] principle *)
-Lemma euttge_trans_clo_wcompat E1 E2 R1 R2 (REv : forall A B, E1 A -> E2 B -> Prop)
-      (RAns : forall A B, E1 A -> A -> E2 B -> B -> Prop ) (RR : R1 -> R2 -> Prop) :
-  wcompatible2 (rutt_ REv RAns RR) (euttge_trans_clo RR).
-Proof.
-  constructor; eauto with paco.
-  { red. intros. eapply euttge_trans_clo_mon; eauto. }
-  intros.
-  destruct PR. punfold EQVl. punfold EQVr. unfold_eqit.
-  hinduction REL before r; intros; clear t1' t2'.
-  - remember (RetF r1) as x. red.
-    hinduction EQVl before r; intros; subst; try inv Heqx; eauto; (try constructor; eauto).
-    remember (RetF r3) as x. hinduction EQVr before r; intros; subst; try inv Heqx; (try constructor; eauto).
-  - red. remember (TauF m1) as x.
-    hinduction EQVl before r; intros; subst; try inv Heqx; try inv CHECK; ( try (constructor; eauto; fail )).
-    remember (TauF m3) as y.
-    hinduction EQVr before r; intros; subst; try inv Heqy; try inv CHECK; (try (constructor; eauto; fail)).
-    pclearbot. constructor. gclo. econstructor; eauto with paco.
-  - remember (VisF e1 k1) as x. red.
-    hinduction EQVl before r; intros; subst; try discriminate; try (constructor; eauto; fail).
-    remember (VisF e2 k3) as y.
-    hinduction EQVr before r; intros; subst; try discriminate; try (constructor; eauto; fail).
-    dependent destruction Heqx.
-    dependent destruction Heqy.
-    constructor; auto. intros. apply H0 in H1. pclearbot.
-    apply gpaco2_clo.
-    econstructor; eauto with itree.
-  - remember (TauF t1) as x. red.
-    hinduction EQVl before r; intros; subst; try inv Heqx; try inv CHECK; (try (constructor; eauto; fail)).
-    pclearbot. punfold REL. constructor. eapply IHREL; eauto.
-  - remember (TauF t2) as y. red.
-    hinduction EQVr before r; intros; subst; try inv Heqy; try inv CHECK; (try (constructor; eauto; fail)).
-    pclearbot. punfold REL. constructor. eapply IHREL; eauto.
-Qed.
-
-#[global] Hint Resolve euttge_trans_clo_wcompat : paco.
-
-(* The validity of the up-to [euttge] entails we can rewrite under [euttge]
-   and hence also [eq_itree] during coinductive proofs of [rutt]
-*)
-#[global] Instance grutt_cong_eqit {R1 R2 : Type} {E1 E2 : Type -> Type} {REv : forall A B, E1 A -> E2 B -> Prop}
-       {RAns : forall A B, E1 A -> A -> E2 B -> B -> Prop} {RR1 RR2} {RS : R1 -> R2 -> Prop} r rg
-       (LERR1: forall x x' y, (RR1 x x': Prop) -> (RS x' y: Prop) -> RS x y)
-       (LERR2: forall x y y', (RR2 y y': Prop) -> RS x y' -> RS x y) :
-  Proper (eq_itree RR1 ==> eq_itree RR2 ==> flip impl)
-         (gpaco2 (rutt_ REv RAns RS) (euttge_trans_clo RS) r rg).
-Proof.
-  repeat intro. gclo. econstructor; eauto;
-    try eapply eqit_mon; try apply H; try apply H0; auto.
-Qed.
-
-Global Instance grutt_cong_euttge {R1 R2 : Type} {E1 E2 : Type -> Type} {REv : forall A B, E1 A -> E2 B -> Prop}
-       {RAns : forall A B, E1 A -> A -> E2 B -> B -> Prop} {RR1 RR2} {RS : R1 -> R2 -> Prop} r rg
-       (LERR1: forall x x' y, (RR1 x x': Prop) -> (RS x' y: Prop) -> RS x y)
-       (LERR2: forall x y y', (RR2 y y': Prop) -> RS x y' -> RS x y) :
-  Proper (euttge RR1 ==> euttge RR2 ==> flip impl)
-         (gpaco2 (rutt_ REv RAns RS) (euttge_trans_clo RS) r rg).
-Proof.
-  repeat intro. gclo. econstructor; eauto.
-Qed.
-
-(* Provide these explicitly since typeclasses eauto cannot infer them *)
-
-#[global] Instance grutt_cong_eqit_eq {R1 R2 : Type} {E1 E2 : Type -> Type} {REv : forall A B, E1 A -> E2 B -> Prop}
-      {RAns : forall A B, E1 A -> A -> E2 B -> B -> Prop} {RS : R1 -> R2 -> Prop} r rg:
-    Proper (eq_itree eq ==> eq_itree eq ==> flip impl)
-         (gpaco2 (rutt_ REv RAns RS) (euttge_trans_clo RS) r rg).
-Proof.
-  apply grutt_cong_eqit; now intros * ->.
-Qed.
-
-#[global] Instance grutt_cong_euttge_eq {R1 R2 : Type} {E1 E2 : Type -> Type} {REv : forall A B, E1 A -> E2 B -> Prop}
-      {RAns : forall A B, E1 A -> A -> E2 B -> B -> Prop} {RS : R1 -> R2 -> Prop} r rg:
-    Proper (euttge eq ==> euttge eq ==> flip impl)
-         (gpaco2 (rutt_ REv RAns RS) (euttge_trans_clo RS) r rg).
-Proof.
-  apply grutt_cong_euttge; now intros * ->.
-Qed.
